hol-light/hol_verificationScript.sml
@@ -1,0 +1,140 @@
+
+open HolKernel Parse boolLib bossLib;
+
+val _ = new_theory "hol_verification";
+
+open hol_kernelTheory model_syntaxTheory;
+open listTheory arithmeticTheory combinTheory pairTheory;
+
+open monadsyntax;
+val _ = temp_overload_on ("monad_bind", ``ex_bind``);
+val _ = temp_overload_on ("return", ``ex_return``);
+val _ = set_trace "Unicode" 0;
+
+infix \\ val op \\ = op THEN;
+
+(* ------------------------------------------------------------------------- *)
+(* Translations from implementation types to model types.                    *)
+(* ------------------------------------------------------------------------- *)
+
+val MEM_hol_type_size = prove(
+  ``!tys a. MEM a tys ==> hol_type_size a < hol_type1_size tys``,
+  Induct \\ SIMP_TAC std_ss [MEM,hol_type_size_def] \\ REPEAT STRIP_TAC
+  \\ FULL_SIMP_TAC std_ss [] \\ RES_TAC \\ FULL_SIMP_TAC std_ss [] \\ DECIDE_TAC);
+
+val hol_ty_def = tDefine "hol_ty" `
+  (hol_ty (hol_kernel$Tyvar v) = Tyvar v) /\
+  (hol_ty (Tyapp s tys) =
+     if (s = "bool") /\ (tys = []) then Bool else
+     if (s = "ind") /\ (tys = []) then Ind else
+     if (s = "fun") /\ (LENGTH tys = 2) then
+       Fun (hol_ty (EL 0 tys)) (hol_ty (EL 1 tys))
+     else Tyapp s (MAP hol_ty tys))`
+ (WF_REL_TAC `measure hol_type_size`
+  \\ REPEAT STRIP_TAC
+  \\ IMP_RES_TAC MEM_hol_type_size \\ TRY DECIDE_TAC
+  \\ Cases_on `tys` \\ FULL_SIMP_TAC (srw_ss()) []
+  \\ Cases_on `t` \\ FULL_SIMP_TAC (srw_ss()) []
+  \\ Cases_on `t'` \\ FULL_SIMP_TAC (srw_ss()) [hol_type_size_def]
+  \\ DECIDE_TAC);
+
+val _ = temp_overload_on("fun",``\x y. hol_kernel$Tyapp "fun" [x;y]``);
+val _ = temp_overload_on("bool_ty",``hol_kernel$Tyapp "bool" []``);
+val _ = temp_overload_on("impossible_term",``Const "=" Ind``);
+
+val hol_tm_def = Define `
+  (hol_tm (Var v ty) = Var v (hol_ty ty)) /\
+  (hol_tm (Const s ty) =
+     if s = "=" then
+       if (?a. ty = fun a (fun a bool_ty))
+       then Equal (domain (hol_ty ty))
+       else impossible_term
+     else
+     if s = "@" then
+       if (?a. ty = fun (fun a bool_ty) a)
+       then Select (codomain (hol_ty ty))
+       else impossible_term
+     else
+       Const s (hol_ty ty)) /\
+  (hol_tm (Comb x y) = Comb (hol_tm x) (hol_tm y)) /\
+  (hol_tm (Abs (Var v ty) x) = Abs v (hol_ty ty) (hol_tm x)) /\
+  (hol_tm _ = impossible_term)`;
+
+val hol_ctxt_def = Define `
+  (hol_ctxt [] = []) /\
+  (hol_ctxt (Axiomdef tm::ctxt) =
+    (Axiomdef (hol_tm tm)) :: hol_ctxt ctxt) /\
+  (hol_ctxt (Constdef n tm::ctxt) =
+    (Constdef n (hol_tm tm)) :: hol_ctxt ctxt) /\
+  (hol_ctxt (Typedef s1 tm s2 s3 :: ctxt) =
+    (Typedef s1 (hol_tm tm) s2 s3) :: hol_ctxt ctxt)`;
+
+(* ------------------------------------------------------------------------- *)
+(* type_ok, term_ok, context_ok and |- for implementation types.             *)
+(* ------------------------------------------------------------------------- *)
+
+val TYPE_def = Define `
+  TYPE ctxt ty = type_ok (hol_ctxt ctxt) (hol_ty ty)`;
+
+val TERM_def = Define `
+  TERM ctxt tm = welltyped_in (hol_tm tm) (hol_ctxt ctxt)`;
+
+val CONTEXT_def = Define `
+  CONTEXT ctxt = context_ok (hol_ctxt ctxt)`;
+
+val THM_def = Define `
+  THM ctxt (Sequent asl c) = ((MAP hol_tm asl, hol_ctxt ctxt) |- hol_tm c)`;
+
+(* ------------------------------------------------------------------------- *)
+(* Certain terms cannot occur                                                *)
+(* ------------------------------------------------------------------------- *)
+
+val NOT_EQ_CONST = prove(
+  ``!ctxt x. context_ok (hol_ctxt ctxt) ==>
+             ~MEM ("=",x) (consts (hol_ctxt ctxt))``,
+  Induct \\ FULL_SIMP_TAC std_ss [consts,MAP,FLAT,MEM,hol_ctxt_def]
+  \\ Cases \\ FULL_SIMP_TAC std_ss [consts,MAP,FLAT,MEM,hol_ctxt_def]
+  \\ FULL_SIMP_TAC std_ss [consts_aux,APPEND,MEM,context_ok,def_ok]
+  \\ FULL_SIMP_TAC std_ss [reserved_const_names,MEM]);
+
+val impossible_term_thm = prove(
+  ``TERM ctxt tm ==> hol_tm tm <> impossible_term ``,
+  SIMP_TAC std_ss [TERM_def,welltyped_in] \\ REPEAT STRIP_TAC
+  \\ FULL_SIMP_TAC std_ss [term_ok] \\ IMP_RES_TAC NOT_EQ_CONST);
+
+val Abs_Var = prove(
+  ``TERM ctxt (Abs v tm) ==> ?s ty. v = Var s ty``,
+  REPEAT STRIP_TAC \\ IMP_RES_TAC impossible_term_thm
+  \\ Cases_on `v` \\ FULL_SIMP_TAC (srw_ss()) [hol_tm_def]);
+
+val Equal_type = prove(
+  ``TERM ctxt (Const "=" ty) ==> ?a. ty = fun a (fun a bool_ty)``,
+  REPEAT STRIP_TAC \\ IMP_RES_TAC impossible_term_thm
+  \\ FULL_SIMP_TAC std_ss [hol_tm_def] \\ METIS_TAC []);
+
+val Select_type = prove(
+  ``TERM ctxt (Const "@" ty) ==> ?a. ty = fun (fun a bool_ty) a``,
+  REPEAT STRIP_TAC \\ IMP_RES_TAC impossible_term_thm
+  \\ FULL_SIMP_TAC std_ss [hol_tm_def,EVAL ``"@" = "="``] \\ METIS_TAC []);
+
+(* ------------------------------------------------------------------------- *)
+(* State invariant                                                           *)
+(* ------------------------------------------------------------------------- *)
+
+
+
+(*
+
+type_ok_CASES
+term_ok
+REFL_def
+mk_eq_def
+mk_const_def
+mk_comb_def
+type_of_def
+typeof
+proves_RULES
+
+*)
+
+val _ = export_theory();
